

Derivation of Faulhbar's Formula

Ojas Kalra

April 19, 2023



$$1 + 2 + 3 + \dots + n = n(n+1)/2$$



$$1^2 + 2^2 + 3^2 + \dots + n^2 = n(n+1)(2n+1)/6$$



$$1^3 + 2^3 + 3^3 + \dots + n^3 = n^2(n+1)^2/4$$



$$1^p + 2^p + 3^p + \dots + n^p = ?$$

Derivation

► Let

$$G(x) = 1 + e^x + e^{2x} + e^{3x} + \dots e^{nx} = \frac{e^{(n+1)x} - 1}{e^x - 1} \quad x \neq 0$$

► Note

$$G'(0) = 1 + 2 + 3 \dots n$$

$$G^{(2)}(0) = 1^2 + 2^2 + 3^2 \dots + n^2$$

$$G^{(3)}(0) = 1^3 + 2^3 + 3^3 \dots + n^3$$

$$G^{(p)}(0) = 1^p + 2^p + 3^p \dots + n^p$$

Derivation

Let

$$G'(0) = S_1(n) = 1 + 2 + 3 + \dots + n$$

$$G''(0) = S_2(n) = 1^2 + 2^2 + 3^2 + \dots + n^2$$

$$G'''(0) = S_3(n) = 1^3 + 2^3 + 3^3 + \dots + n^3$$

$$G^{(p)}(0) = S_p(n) = 1^p + 2^p + 3^p + \dots + n^p$$

Using Taylor series expansion of $G(x)$, we get

$$G(x) = S_0(n) + S_1(n) \cdot \frac{x}{1!} + S_2(n) \cdot \frac{x^2}{2!} + S_3(n) \cdot \frac{x^3}{3!} + \dots + S_p(n) \cdot \frac{x^p}{p!} \dots$$

Where

$$S_p(n) = 1^p + 2^p + 3^p + \dots + n^p$$

Derivation

Remember

$$G(x) = \frac{x}{e^x - 1} \cdot \frac{e^{Nx-1}}{x} \text{ where } N = n + 1 \text{ and } x \neq 0$$

Note, now we have the product of two sequences:

$$\frac{x}{e^x - 1} = B_0 + B_1 \frac{x}{1!} + B_2 \frac{x^2}{2!} + B_3 \frac{x^3}{3!} \dots$$

$$\frac{e^{Nx-1}}{x} = N + N^2 \frac{x}{2!} + N^3 \frac{x^2}{3!} + N^4 \frac{x^3}{4!} \dots$$

Derivation

We want to combine these two products

$$\frac{x}{e^x - 1} = B_0 + B_1 \frac{x}{1!} + B_2 \frac{x^2}{2!} + B_3 \frac{x^3}{3!} \dots$$

$$\frac{e^{Nx} - 1}{x} = N + N^2 \frac{x}{2!} + N^3 \frac{x^2}{3!} + N^4 \frac{x^3}{4!} \dots$$

$$(B_0 + B_1 \frac{x}{1!} + B_2 \frac{x^2}{2!} + B_3 \frac{x^3}{3!} \dots) \cdot (N + N^2 \frac{x}{2!} + N^3 \frac{x^2}{3!} + N^4 \frac{x^3}{4!} \dots)$$

We want to match all the terms in the form $\frac{x^j}{j!}$ so we can use...

Theorem (Cauchy Product of Power Series)

$$\left(\sum_{k=0}^{\infty} a_k \cdot \frac{x^k}{k!} \right) \cdot \left(\sum_{m=0}^{\infty} b_m \cdot \frac{x^m}{m!} \right) = \sum_{k=0}^{\infty} \sum_{m=0}^k \binom{k}{m} a_m \cdot b_{k-m} \cdot \frac{x^k}{k!}$$

Derivation

Note

$$N + N^2 \frac{x}{2!} + N^3 \frac{x^2}{3!} + N^4 \frac{x^3}{4!} \dots = \frac{1}{x} \sum_{m=1}^{\infty} N^m \cdot \frac{x^m}{m!}$$

So our product

$$(B_0 + B_1 \frac{x}{1!} + B_2 \frac{x^2}{2!} + B_3 \frac{x^3}{3!} \dots) \cdot (N + N^2 \frac{x}{2!} + N^3 \frac{x^2}{3!} + N^4 \frac{x^3}{4!} \dots)$$

is the same as

$$\left(\sum_{k=0}^{\infty} B_k \cdot \frac{x^k}{k!} \right) \cdot \left(\sum_{m=1}^{\infty} N^m \cdot \frac{x^m}{m!} \right) \cdot \frac{1}{x}$$

Derivation

We still can't apply our theorem (Cauchy Product of Power Series) because

$$\frac{1}{x} \left(\sum_{k=0}^{\infty} B_k \frac{x^k}{k!} \right) \left(\sum_{m=1}^{\infty} N^m \frac{x^m}{m!} \right)$$

has the bounds $m = 1$ to infinity. We want it to start at $m = 0$. Note, our series is

$$\frac{1}{x} \left(B_0 + B_1 \frac{x}{1!} + B_2 \frac{x^2}{2!} + B_3 \frac{x^3}{3!} \dots \right) \left(N + N^2 \frac{x^2}{2!} + N^3 \frac{x^3}{3!} + N^4 \frac{x^4}{4!} \dots \right)$$

Collecting like terms for $x \dots$

$$\frac{1}{x} \left(\left(B_0 \frac{x^0}{0!} N^1 \frac{x^1}{1!} \right) + \left(B_0 \frac{x^0}{0!} N^2 \frac{x^2}{2!} + B_1 \frac{x^1}{1!} N \frac{x^1}{1!} \right) + \dots \right)$$

Derivation

$$\begin{aligned} & \frac{1}{x} \left(\sum_{k=0}^{\infty} B_k \frac{x^k}{k!} \right) \left(\sum_{m=1}^{\infty} N^m \frac{x^m}{m!} \right) \\ &= \frac{1}{x} \left(\left(B_0 \frac{x^0}{0!} N^1 \frac{x^1}{1!} \right) + \left(B_0 \frac{x^0}{0!} N^2 \frac{x^2}{2!} + B_1 \frac{x^1}{1!} N \frac{x^1}{1!} \right) + \dots \right) \end{aligned}$$

Note the term

$$\left(B_k \frac{x^k}{k!} \cdot N^0 \frac{x^0}{0!} \right)$$

never appears, thus

$$\frac{1}{x} \sum_{k=1}^{\infty} \sum_{m=0}^{k-1} \binom{k}{m} B_m N^{k-m} \frac{x^k}{k!}$$

Derivation

$$\frac{1}{x} \sum_{k=1}^{\infty} \sum_{m=0}^{k-1} \binom{k}{m} B_m N^{k-m} \frac{x^k}{k!}$$

let $n = k - 1$

$$\begin{aligned} & \frac{1}{x} \left(\sum_{n=0}^{\infty} \sum_{m=0}^n \binom{n+1}{m} B_m N^{n+1-m} \frac{x^{n+1}}{(n+1)!} \right) \\ &= \sum_{n=0}^{\infty} \sum_{m=0}^n \binom{n+1}{m} \frac{B_m N^{n+1-m}}{n+1} \frac{x^n}{n!} \\ &= \sum_{n=0}^{\infty} \sum_{m=0}^n \binom{n+1}{m} \frac{B_m N^{n+1-m}}{n+1} \frac{x^n}{n!} \end{aligned}$$

Derivation

As of now, we have

$$S_p(n) = G^{(p)}(0) = \frac{1}{p+1} \sum_{p=0}^{\infty} \sum_{m=0}^p \binom{p+1}{m} B_m N^{p+1-m} \frac{x^p}{p!}$$

Note

$$\begin{aligned} S_p(N) &= S_p(n) + N^p = \frac{1}{p+1} \sum_{m=0}^p \binom{p+1}{m} B_m N^{p+1-m} + N^p \\ &= \frac{1}{p+1} \left(\binom{p+1}{0} B_0 N^{p+1} + \binom{p+1}{1} B_1 N^p + \binom{p+1}{2} B_2 N^{p-1} + \dots \right) \\ &\quad + N^p \end{aligned}$$

Derivation

$$S_p(N) = \frac{1}{p+1} \left(\binom{p+1}{0} B_0 N^{p+1} + \binom{p+1}{1} B_1 N^p + \right. \\ \left. \binom{p+2}{2} B_2 N^{p-1} + \dots \right) + N^p$$

Note

$$B_i = 0 \quad \forall \text{ odd } i > 1$$

and

$$B_1 = -\frac{1}{2} = -1 - B_1$$

Combining the

N^p term with $\frac{1}{p+1} \cdot \binom{p+1}{1} B_1 N^p$, we get $-N^p - B_1 N^p + N^p = -B_1 N^p$. Thus we can write,

$$S_p(N) = \frac{1}{p+1} \sum_{j=0}^p (-1)^j \binom{p+1}{j} B_j N^{p+1-j}$$

Conclusion

A closed form for $1^p + 2^p + 3^p \dots + n^p$

is

$$\frac{1}{p+1} \sum_{j=0}^p (-1)^j \binom{p+1}{j} B_j N^{p+1-j}$$

Thank You

Thank you for listening!

Questions?